prove i1 not ioco s3

examples/IOTS_ex.v
@@ -1,3 +1,4 @@
+Require Import IOCO.
 Require Import BE_ltacs.
 Require Import String.
 Require Import Coq.Lists.List.
@@ -147,6 +148,117 @@ Proof.
       * apply one_step_reachability_r1 with (s1 := 3) (s2 := 3);
         try (apply empty_reachability_r1). apply transition_r1. elem_in_list.
       * apply seq_reachability_r1. apply empty_reachability_r1.
+Defined.
+
+Definition spec_s1_LTS : LTS.
+Proof.
+  solve_LTS_rules
+    [1;2;3]
+    ["a";"x"]
+    [(1, event "a", 2);(2, event "x", 3)]
+    1.
+Defined.
+
+Definition spec_s1_SC_LTS : SC_LTS.
+Proof.
+ apply (mkSC_LTS spec_s1_LTS).
+ unfold strongly_converging. intros s t H. destruct t.
+  - destruct H. unfold not in H. exfalso. apply H. reflexivity.
+  - unfold all_labels_tau in H. destruct H as [_ [H _]].
+    unfold not. intros H'. inversion H'.
+    + subst. proof_absurd_transition H5.
+    + subst. explore_transition H3.
+Defined.
+
+Definition spec_s1_IOLTS : IOLTS.
+Proof.
+  solve_IOLTS_rules
+    spec_s1_SC_LTS
+    ["a"]
+    ["x"].
+Defined.
+
+(*
+
+Theorem i1_ioco_s1 : ind_ioco imp_i1 spec_s1_IOLTS.
+Proof.
+  unfold ind_ioco. simpl. intros Qi Qs t out_i out_s H.
+  unfold ind_s_traces_LTS in H. unfold ind_s_traces in H. destruct H as [s' H].
+  simpl in H. inversion H; subst.
+  - clear. intros H1 H2. unfold ind_s_after_LTS in H2. simpl in H2. unfold ind_s_after in H2.
+    intros H3 H4. unfold ind_out in H4. intros l H'.
+    assert (H'': forall s, In s Qs -> In l out_s).
+    { intros s H. remember H as H_new. clear HeqH_new. apply H2 in H.
+      inversion H. subst. inversion H0.
+      - subst. simpl in *. specialize (H4 l). destruct H4 as [_ H4].
+        apply H4 in H_new. destruct H_new as [so' [H_new1 H_new2]].
+        inversion H_new1; subst.
+        +
+    
+    }
+    apply H''.
+
+
+
+
+
+  unfold ind_ioco. simpl. intros Qi Qs t out_i out_s H1 H2 H3 H4 H5.
+  unfold incl. intros l. intros H6. destruct l.
+  - admit.
+  - unfold ind_out in H4. specialize (H4 delta).
+    destruct H4 as [H4 _]. apply H4 in H6. clear H4. destruct H6 as [s [so' H6]].
+    destruct H6 as [H6_1 [H6_2 H6_3]]. inversion H6_2; subst.
+    + unfold ind_out in H5. specialize (H5 delta). destruct H5 as [_ H5].
+      unfold ind_s_after_LTS in H3. unfold ind_s_after in H3. simpl in H3.
+  unfold ind_out in H4. specialize (H4 l).
+  destruct H4 as [H4 _]. apply H4 in H6. clear H4. destruct H6 as [s [so' H6]].
+  destruct H6 as [H6_1 [H6_2 H6_3]]. inversion H6_2; subst.
+  - admit.
+  - simpl in H4. unfold ind_out in H5. specialize (H5 l). destruct H5 as [_ H5].
+    unfold ind_s_after_LTS in H3. unfold ind_s_after in H3. simpl in H3.
+  
+  
+  
+  
+  unfold ind_s_traces_LTS in H1.
+  unfold ind_s_traces in H1. destruct H1 as [s' H1].
+  simpl in H1. inversion H1; subst.
+  - unfold ind_s_after_LTS in H2. unfold ind_s_after in H2. simpl in H2.
+    unfold ind_s_after_LTS in H3. unfold ind_s_after in H3. simpl in H3.
+    unfold ind_out in H4. apply H4 in H6. destruct H6 as [s [so' H6]].
+    destruct H6 as [ [H6_1 [H6_2 H6_3]] _]. clear H4. inversion H6_2. 
+    + subst. simpl in H0.
+  unfold ind_s_after_LTS in H2. unfold ind_s_after in H2. specialize (H2 x).
+   unfold ind_s_after_LTS in H3. unfold ind_s_after in H3. specialize (H3 x).
+   apply H3 in H1. unfold ind_out in H5. specialize (H5 a). 
+   -
+*)
+Definition spec_s3_LTS : LTS.
+Proof.
+  solve_LTS_rules
+    [1;2;3;4;5]
+    ["a";"b";"x";"y"]
+    [(1, event "a", 2);(2, event "x", 3);(1, event "b", 4);(4, event "y", 5)]
+    1.
+Defined.
+
+Definition spec_s3_SC_LTS : SC_LTS.
+Proof.
+ apply (mkSC_LTS spec_s3_LTS).
+ unfold strongly_converging. intros s t H. destruct t.
+  - destruct H. unfold not in H. exfalso. apply H. reflexivity.
+  - unfold all_labels_tau in H. destruct H as [_ [H _]].
+    unfold not. intros H'. inversion H'.
+    + subst. proof_absurd_transition H5.
+    + subst. explore_transition H3.
+Defined.
+
+Definition spec_s3_IOLTS : IOLTS.
+Proof.
+  solve_IOLTS_rules
+    spec_s3_SC_LTS
+    ["a";"b"]
+    ["x";"y"].
 Defined.
 
 Local Close Scope string.
